SplinterCache/FunctorParty.s.dfy
@@ -1,0 +1,108 @@
+abstract module UIfc {
+  type UIOp(==)
+}
+
+abstract module UIStateMachine(Ifc:UIfc) {
+  type Vars(==, !new)
+  predicate Init(s:Vars)
+  predicate Next(s:Vars, s':Vars, uiop:Ifc.UIOp)
+}
+
+// The "unwinding condition" necessary to prove the TLA expression:
+// L.Init && []L.Next ==> H.Init && []H.Next
+abstract module StateMachinesRefine(Ifc: UIfc, L:UIStateMachine(Ifc), H:UIStateMachine(Ifc)) {
+
+  // Implementation must supply an interpretation function.
+  function I(s:L.Vars) : H.Vars
+
+  // Implementation provides an invariant to support induction.
+  predicate Inv(s:L.Vars)
+
+  lemma InterpPreservesInit(s:L.Vars)
+      requires L.Init(s)
+      ensures H.Init(I(s))
+
+  lemma InvInit(s:L.Vars)
+      requires L.Init(s)
+      ensures Inv(s)
+
+  lemma InvNext(s:L.Vars, s':L.Vars)
+      requires Inv(s)
+      requires L.Next(s, s')
+      ensures Inv(s')
+      ensures H.Next(I(s), I(s'))
+}
+
+// This module is just a type-template parameter placeholder.
+abstract module BlockType {
+  type Block(==)
+}
+
+abstract module BlockIfc(B : BlockType) {
+  type Addr(==)
+  datatype SingletonBlockOp = Read(a:Addr, b:B) | Write(a:Addr, b:B)
+  datatype BlockOp = seq<SingletonBlockOp>
+
+  // IOSystem demands that IOs be one-at-a-time to make room for crashes.
+  SingleIO(dop:BlockOp) { |dop| == 1 }
+}
+
+abstract module DiskProgram(Ifc : UIfc, B : BlockType) {
+  import BlockIfc(B = B)
+
+  type Vars(==, !new)
+  // TODO could we declare that type Vars has these predicates as namespace predicates? That'd be keen.
+  predicate Init(s:Vars)
+  predicate Next(s:Vars, s':Vars, uiop:Ifc.UIOp, dop:BlockOp)
+}
+
+// TODOiscuss with chris: Having to cart around every parameter required by
+// higher-level modules is tedious; it reeks of D<B<A>, C> nonsense in
+// templateland. Would some sort of module-synonym mechanism let us stop doing
+// this? Or should we consider trying to mix these functors with "import :"
+// type abstraction from Dafny (which still confuses me easily)? I mean, it
+// SHOULD help, because instead of a takes-a relation, we'd use a has-a relation.
+// Happy to try it, but suspicious we'll be unable to fill in those holes later
+// to make them match other parameters. Try it with me?
+module IOSystem(Ifc: Ifc, B: BlockType, Program : DiskProgram(Ifc, B))
+  refines UIStateMachine(Ifc = Ifc)
+{
+  datatype Vars = Vars(p: Program.Vars, d: Disk.Vars)
+
+  predicate Init(s:Vars)
+  {
+    && Program.Init(s.p)
+    && Program.Mkfs(s.d)
+  }
+
+  predicate Next(s:Vars, s':Vars, uiop:Ifc.UIOp)
+  {
+    // XXX add crash steps
+    exists dop ::
+    && SingleIO(dop)
+    && Program.Next(s.p, s'.p, uiop, dop)
+    && Disk.Next(s.d, s'.d, dop)
+  }
+}
+
+
+// .s This is the climax of the system. Build system demands that it be instantiatied
+// as a non-abstract module, hence supplying a proof.
+abstract module SystemTheorem(
+  Ifc: UIfc, B: BlockType, P: DiskProgram(Ifc = Ifc, B = B), CrashSafeSpec: UIStateMachine(Ifc = Ifc),
+  Proof : StateMachinesRefine(
+    L = IOSystem(DiskProgram = P),
+    H = CrashSafeSpec)))
+
+//////////////////////////////////////////////////////////////////////////////
+
+// XXX TODO As written above, nothing forces CrashSafeSpec to actually be
+// CrashSafe(Map), nor does anything force P to be
+// CachedStorageSystem(CacheClient = Betree, Cache = CrashSafeCache).  Does
+// that binding belong in a more-detailed theorem here in this .s, or is that a
+// build-system constraint?
+//
+// Maybe the code above is a library .s file, and then another .s file would
+// bring in Map and CrashSafe to provide the actual Theorem for our particular
+// system.  The build system would be what demands the match between the impl
+// and whatever spec we're offering in impl (Betree + CrashSafeCache).
